src/ByteStringHeap.v
@@ -1,0 +1,350 @@
+Require Import
+  Coq.Lists.List
+  Coq.Arith.Arith
+  Coq.NArith.NArith
+  Fiat.ADT
+  Fiat.ADTNotation
+  Fiat.ADTRefinement
+  Fiat.ADTRefinement.BuildADTRefinements
+  ByteString.ADTInduction
+  ByteString.BindDep
+  ByteString.ByteString
+  ByteString.Heap
+  ByteString.HeapADT
+  ByteString.Nomega
+  ByteString.Relations
+  ByteString.Tactics
+  ByteString.TupleEnsembles
+  ByteString.Within.
+
+Generalizable All Variables.
+
+Open Scope N_scope.
+
+(*
+Lemma within_index : forall addr len i,
+  (i <? len) -> within addr len (addr + i).
+Proof.
+  intros.
+  split.
+    apply N.le_add_r.
+  apply N.add_lt_mono_l.
+  apply N.ltb_lt.
+  assumption.
+Qed.
+*)
+
+Module ByteStringHeap (Mem : Memory).
+
+Module Import BS := ByteString Mem.
+Module Import Adt := HeapADT Mem.
+Import Heap.
+
+Definition HSpec := projT1 HeapSpecADT.
+
+Definition memcpy' (r : Rep HSpec) (addr : N) (addr2 : N) (len : N) :
+  Comp (Rep HSpec * unit) :=
+  Eval simpl in callMeth HSpec memcpyS r addr addr2 len.
+
+Definition realloc' (r : Rep HSpec) (addr : N) (len : N | 0 < len) :
+  Comp (Rep HSpec * N) :=
+  Eval simpl in callMeth HSpec reallocS r addr len.
+
+Definition peek' (r : Rep HSpec) (addr : N) :
+  Comp (Rep HSpec * Mem.Word8) :=
+  Eval simpl in callMeth HSpec peekS r addr.
+
+Definition poke' (r : Rep HSpec) (addr : N) (w : Mem.Word8) :
+  Comp (Rep HSpec * unit) :=
+  Eval simpl in callMeth HSpec pokeS r addr w.
+
+Record PS := makePS {
+  psHeap : Rep HSpec;
+
+  psBuffer : N;
+  psBufLen : N;
+
+  psOffset : N;
+  psLength : N
+}.
+
+Record Correct (ps : PS) : Prop := {
+  _ : psOffset ps + psLength ps <= psBufLen ps;
+  _ : 0 < psBufLen ps -> exists data,
+        Lookup (psBuffer ps) {| memSize := psBufLen ps
+                              ; memData := data |} (` (psHeap ps))
+}.
+
+Theorem Nlt_plus_1 : forall n : N, 0 < n + 1.
+Proof. nomega. Qed.
+
+Definition buffer_cons (r : PS) (d : Mem.Word8) : Comp PS :=
+  ps <- If 0 <? psOffset r
+        Then ret {| psHeap   := psHeap r
+                  ; psBuffer := psBuffer r
+                  ; psBufLen := psBufLen r
+                  ; psOffset := psOffset r - 1
+                  ; psLength := psLength r + 1 |}
+        Else If psLength r <? psBufLen r
+        Then (
+          res <- memcpy' (psHeap r) (psBuffer r) (psBuffer r + 1)
+                         (psLength r);
+          ret {| psHeap   := fst res
+               ; psBuffer := psBuffer r
+               ; psBufLen := psBufLen r
+               ; psOffset := 0
+               ; psLength := psLength r + 1 |})
+        Else (
+          (* jww (2016-06-28): We could make a trade-off here by allocating
+             extra bytes at the beginning in anticipation of future calls to
+             [buffer_cons]. *)
+          res <- realloc' (psHeap r) (psBuffer r)
+                          (exist _ (psLength r + 1) (Nlt_plus_1 _));
+          ret {| psHeap   := fst res
+               ; psBuffer := snd res
+               ; psBufLen := psLength r + 1
+               ; psOffset := 0
+               ; psLength := psLength r + 1 |});
+  res <- poke' (psHeap ps) (psBuffer ps + psOffset ps) d;
+  ret {| psHeap   := fst res
+       ; psBuffer := psBuffer ps
+       ; psBufLen := psBufLen ps
+       ; psOffset := psOffset ps
+       ; psLength := psLength ps |}.
+
+Lemma refine_ret_eq_r : forall A (a b : A), refine (ret a) (ret b) -> a = b.
+Proof.
+  intros.
+  specialize (H b (ReturnComputes b)).
+  apply Return_inv; assumption.
+Qed.
+
+Theorem If_Then_Else_correct :
+  forall b cpst cpse ps',
+    (forall pst, b = true -> refine cpst (ret pst) -> Correct pst) ->
+    (forall pse, b = false -> refine cpse (ret pse) -> Correct pse) ->
+    refine (If b
+            Then cpst
+            Else cpse) (ret ps') -> Correct ps'.
+Proof.
+  intros.
+  specialize (H1 ps' (ReturnComputes ps')).
+  destruct b; simpl in *;
+  [ apply H | apply H0 ]; auto;
+  intros ??;
+  apply Return_inv in H2; subst;
+  assumption.
+Qed.
+
+Theorem poke'_correct `(_ : Correct ps) : forall offset length d ps',
+  0 < length ->
+  offset + length <= psBufLen ps ->
+  refine (res <- poke' (psHeap ps) (psBuffer ps + offset) d;
+          ret {| psHeap   := fst res
+               ; psBuffer := psBuffer ps
+               ; psBufLen := psBufLen ps
+               ; psOffset := offset
+               ; psLength := length |}) (ret ps') -> Correct ps'.
+Proof.
+  intros ??????.
+  unfold poke', poke.
+  rewrite refine_bind_dep_bind_ret; simpl.
+  rewrite refine_bind_dep_ret; simpl.
+  intro H1.
+  apply refine_ret_eq_r in H1.
+  subst; simpl.
+  destruct Correct0.
+  constructor; simpl; [nomega|].
+  intuition; destruct_ex.
+  exists (Update offset d x).
+  teardown.
+  exists {| memSize := psBufLen ps; memData := x |}; simpl.
+  decisions; intuition; f_equal.
+    f_equal; nomega.
+  nomega.
+Qed.
+
+Definition buffer_uncons (r : PS) : Comp (PS * option Mem.Word8) :=
+  If 0 <? psLength r
+  Then (
+    w <- peek' (psHeap r) (psBuffer r + psOffset r);
+    ret ({| psHeap   := psHeap r
+          ; psBuffer := psBuffer r
+          ; psBufLen := psBufLen r
+          ; psOffset := psOffset r + 1
+          ; psLength := psLength r - 1 |}, Some (snd w))
+  )
+  Else ret (r, None).
+
+Global Program Instance refineEquiv_bind_dep : forall A (ca : Comp A) B,
+  Proper (forall_relation
+            (fun x0 : A =>
+               pointwise_relation (refine ca (ret x0)) refineEquiv) ==>
+            (@refineEquiv B))
+         (Bind_dep ca).
+Obligation 1.
+  intros ???.
+  split; intros; intros ??;
+  apply Bind_dep_inv in H0;
+  destruct H0;
+  exists x0;
+  destruct H0;
+  exists x1;
+  eapply H in c; eauto.
+Qed.
+
+Lemma refineEquiv_If_Then_Else_Bind :
+  forall (A B : Type) (i : bool) (t e : Comp A) (b : A -> Comp B),
+    refineEquiv (a <- If i Then t Else e; b a)
+                (If i Then a <- t; b a Else (a <- e; b a)).
+Proof. split; intros; destruct i; reflexivity. Qed.
+
+Theorem buffer_cons_correct `(_ : Correct ps) : forall ps' x,
+  refine (buffer_cons ps x) (ret ps') -> Correct ps'.
+Proof.
+  unfold buffer_cons; intros.
+  revert H.
+  rewrite refineEquiv_If_Then_Else_Bind.
+  apply If_Then_Else_correct; intros ??.
+    autorewrite with monad laws; simpl.
+    apply poke'_correct; trivial.
+      nomega.
+    destruct Correct0.
+    nomega.
+  rewrite refineEquiv_If_Then_Else_Bind.
+  apply If_Then_Else_correct; intros ??.
+    autorewrite with monad laws; simpl.
+    admit.
+  autorewrite with monad laws; simpl.
+  admit.
+Admitted.
+
+Theorem buffer_cons_length_increase ps : forall ps' x,
+  buffer_cons ps x ↝ ps' -> psLength ps' = psLength ps + 1.
+Proof.
+  unfold buffer_cons, peek, poke, memcpy in *.
+  destruct (0 <? psOffset ps) eqn:Heqe;
+  destruct (psLength ps <? psBufLen ps);
+  simpl; intros; clear -H; simpl in H;
+  simplify_ensembles; subst; simpl;
+  reflexivity.
+Qed.
+
+(*
+Theorem buffer_cons_data_retained `(_ : Correct ps) : forall ps' x,
+  buffer_cons ps x ↝ ps' ->
+    (x <- peek (` (psHeap ps')) (psOffset ps'); ret (snd x)) ↝ x /\
+    forall i,
+      refineEquiv
+        (x <- peek (` (psHeap ps')) (psOffset ps' + (i + 1)); ret (snd x))
+        (x <- peek (` (psHeap ps)) (psOffset ps + i); ret (snd x)).
+Proof.
+  unfold buffer_cons, peek, poke, memcpy in *.
+  destruct (0 <? psOffset ps) eqn:Heqe;
+  destruct (psLength ps <? psBufLen ps);
+  simpl; intros; clear -H Heqe; simpl in H;
+  simplify_ensembles; subst; simpl;
+  autorewrite with monad laws;
+  simplify_ensembles; subst; simpl;
+  intros; reduction.
+*)
+
+Definition ByteString_list_AbsR (or : Rep ByteStringSpec) `(nr : PS) :=
+     (* then the list and active region must be the same size *)
+     length or = N.to_nat (psLength nr)
+     (* and for every index within the list... *)
+  /\ forall i, (i <? length or)%nat
+     (* each byte in the list matches its corresponding byte in the buffer. *)
+       -> forall x, x = nth i or x
+          <-> (x <- peek (` (psHeap nr)) (psOffset nr + N.of_nat i);
+               ret (snd x)) ↝ x.
+
+Theorem buffer_cons_sound
+        (r_o : list Mem.Word8) (r_n : PS)
+        (AbsR : ByteString_list_AbsR r_o r_n) :
+  forall x r_n' (H : buffer_cons r_n x ↝ r_n'),
+    ByteString_list_AbsR (x :: r_o) r_n'.
+Proof.
+  intros.
+  split; intros.
+    apply buffer_cons_length_increase in H.
+    destruct AbsR; nomega.
+  split; intros.
+    rewrite H1; clear H1.
+    admit.
+  admit.
+Admitted.
+
+Theorem buffer_uncons_sound
+        (r_o : list Mem.Word8) (r_n : PS)
+        (AbsR : ByteString_list_AbsR r_o r_n) :
+  forall x r_n' (H : buffer_uncons r_n ↝ (r_n', x)),
+    ByteString_list_AbsR (match x with
+                          | None   => r_o
+                          | Some _ => tl r_o
+                          end) r_n'.
+Proof.
+  intros.
+  split; intros.
+    admit.
+  split; intros.
+    admit.
+  admit.
+Admitted.
+
+Lemma ByteStringImpl (heap : Rep HSpec) : FullySharpened ByteStringSpec.
+Proof.
+  start sharpening ADT.
+  hone representation using ByteString_list_AbsR.
+  {
+    simplify with monad laws.
+    refine pick val
+      {| psHeap   := heap
+       ; psBuffer := 0
+       ; psBufLen := 0
+       ; psOffset := 0
+       ; psLength := 0 |}.
+      finish honing.
+    split; intros.
+      reflexivity.
+    split; intros; discriminate.
+  }
+  {
+    simplify with monad laws.
+    etransitivity.
+      eapply (refine_skip2 (dummy:=buffer_cons r_n d)).
+    etransitivity.
+      apply refine_under_bind; intros; simpl.
+      refine pick val a.
+        simplify with monad laws.
+        finish honing.
+      eapply buffer_cons_sound; eauto.
+    unfold buffer_cons.
+    simplify with monad laws; simpl.
+    finish honing.
+  }
+  {
+    simplify with monad laws.
+    etransitivity.
+      eapply (refine_skip2 (dummy:=buffer_uncons r_n)).
+    etransitivity.
+      apply refine_under_bind; intros; simpl.
+      refine pick val (fst a).
+        simplify with monad laws.
+        finish honing.
+      pose proof (buffer_uncons_sound H0 (snd a) (fst a)).
+      rewrite <- surjective_pairing in H2.
+      specialize (H2 H1).
+      destruct a; simpl in *.
+      simpl.
+      admit.
+    unfold buffer_uncons.
+    admit.
+  }
+  finish_SharpeningADT_WithoutDelegation.
+Admitted.
+
+Fail Definition ByteStringImpl' := Eval simpl in projT1 ByteStringImpl.
+(* Print ByteStringImpl'. *)
+
+End ByteStringHeap.
